Merge updated ott generated coq definitions

theories/isla_lang.v
@@ -80,20 +80,6 @@ Inductive binop : Set :=
  | Bvarith (bvarith5:bvarith)
  | Bvcomp (bvcomp5:bvcomp).
 
-Inductive valu : Set := 
- | Val_Symbolic (vvar5:isla_var)
- | Val_Bool (bool5:bool)
- | Val_I (bvi5:Z) (int5:Z)
- | Val_Bits (bv5:string)
- | Val_Enum (enum5:enum)
- | Val_String (str5:string)
- | Val_Unit : valu
- | Val_NamedUnit (name5:register_name)
- | Val_Vector (_:list valu)
- | Val_List (_:list valu)
- | Val_Struct (_:list register_name * valu)
- | Val_Poison : valu.
-
 Inductive accessor : Set := 
  | Field (name5:register_name).
 
@@ -113,7 +99,19 @@ Inductive exp : Set :=
  | Manyop (manyop5:manyop) (_:list exp) (annot5:unit)
  | Ite (exp1:exp) (exp2:exp) (exp3:exp) (annot5:unit).
 
-Definition valu_option : Set := option valu.
+Inductive valu : Set := 
+ | Val_Symbolic (vvar5:isla_var)
+ | Val_Bool (bool5:bool)
+ | Val_I (bvi5:Z) (int5:Z)
+ | Val_Bits (bv5:string)
+ | Val_Enum (enum5:enum)
+ | Val_String (str5:string)
+ | Val_Unit : valu
+ | Val_NamedUnit (name5:register_name)
+ | Val_Vector (_:list valu)
+ | Val_List (_:list valu)
+ | Val_Struct (_:list register_name * valu)
+ | Val_Poison : valu.
 
 Inductive accessor_list : Set := 
  | Nil : accessor_list
@@ -125,25 +123,49 @@ Inductive smt : Set :=
  | Assert (exp5:exp)
  | DefineEnum (int5:Z).
 
+Definition valu_option : Set := option valu.
+
 Inductive event : Set := 
  | Smt (smt5:smt) (annot5:unit)
  | Branch (int5:Z) (str5:string) (annot5:unit) (*r Sail trace fork *)
- | ReadReg (name5:register_name) (accessor_list5:accessor_list) (valu5:valu) (annot5:unit) (*r read register *)
- | WriteReg (name5:register_name) (accessor_list5:accessor_list) (valu5:valu) (annot5:unit) (*r write register *)
- | ReadMem (valu5:valu) (rkind:valu) (addr:valu) (nat5:nat) (tag_value:valu_option) (annot5:unit) (*r read memory *)
- | WriteMem (vvar5:isla_var) (wkind:valu) (addr:valu) (data:valu) (nat5:nat) (tag_value:valu_option) (annot5:unit) (*r write memory *)
- | BranchAddress (addr:valu) (annot5:unit) (*r announce branch address, to induce ctrl dependency in concurrency model *)
- | Barrier (bkind:valu) (annot5:unit) (*r memory barrier *)
- | CacheOp (ckind:valu) (addr:valu) (annot5:unit) (*r cache maintenance effect, for data-cache clean etc. *)
+ | ReadReg (name5:register_name) (accessor_list5:accessor_list) (valu5:valu) (annot5:unit) (*r read value `valu` from register `name` *)
+ | WriteReg (name5:register_name) (accessor_list5:accessor_list) (valu5:valu) (annot5:unit) (*r write value `valu` to register `name` *)
+ | ReadMem (valu5:valu) (rkind:valu) (addr:valu) (num_bytes:nat) (tag_value:valu_option) (annot5:unit) (*r read value `valu` from memory address `addr`, with read kind `rkind`, byte width `byte_width`, and `tag_value` is the optional capability tag *)
+ | WriteMem (vvar5:isla_var) (wkind:valu) (addr:valu) (data:valu) (num_bytes:nat) (tag_value:valu_option) (annot5:unit) (*r write value `valu` to memory address `addr`, with write kind `wkind`, byte width `byte_width`, `tag_value` is the optional capability tag, and success flag `vvar` *)
+ | BranchAddress (addr:valu) (annot5:unit) (*r announce branch address `addr`, to induce ctrl dependency in the concurrency model *)
+ | Barrier (bkind:valu) (annot5:unit) (*r memory barrier of kind `bkind` *)
+ | CacheOp (ckind:valu) (addr:valu) (annot5:unit) (*r cache maintenance effect of kind `ckind`, at address `addr`, for data-cache clean etc. *)
  | MarkReg (name5:register_name) (str5:string) (annot5:unit) (*r instrumentation to tell concurrency model to ignore certain dependencies (TODO: support marking multiple registers). Currently the str is ignore-edge or ignore-write *)
  | Cycle (annot5:unit) (*r instruction boundary *)
- | Instr (opcode:valu) (annot5:unit) (*r records the instruction opcode that was fetched *)
+ | Instr (opcode:valu) (annot5:unit) (*r records the instruction `opcode` that was fetched *)
  | Sleeping (vvar5:isla_var) (annot5:unit) (*r Arm sleeping predicate *)
  | WakeRequest (annot5:unit) (*r Arm wake request *)
  | SleepRequest (annot5:unit) (*r Arm sleep request *).
 
+Inductive valu_concrete : Set := 
+ | CVal_Bool (bool5:bool)
+ | CVal_I (bvi5:Z) (int5:Z)
+ | CVal_Bits (bv5:string)
+ | CVal_Enum (enum5:enum)
+ | CVal_String (str5:string)
+ | CVal_Unit : valu_concrete
+ | CVal_NamedUnit (name5:register_name)
+ | CVal_Vector (_:list valu)
+ | CVal_List (_:list valu)
+ | CVal_Struct (_:list register_name * valu)
+ | CVal_Poison : valu_concrete.
+
 Inductive trc : Set := 
  | Trace (_:list event).
+
+Inductive exp_val : Set := 
+ | EV_Bits (bv5:string) (annot5:unit)
+ | EV_Bool (bool5:bool) (annot5:unit)
+ | EV_Enum (enum5:enum) (annot5:unit)
+ | EV_Unop (unop5:unop) (exp_val5:exp_val) (annot5:unit)
+ | EV_Binop (binop5:binop) (exp_val1:exp_val) (exp_val2:exp_val) (annot5:unit)
+ | EV_Manyop (manyop5:manyop) (_:list exp_val) (annot5:unit)
+ | EV_Ite (exp_val1:exp_val) (exp_val2:exp_val) (exp_val3:exp_val) (annot5:unit).
 (** induction principles *)
 Section exp_rect.
 
@@ -178,6 +200,35 @@ end.
 End exp_rect.
 
 
+Section exp_val_rect.
+
+Variables
+  (P_list_exp_val : list exp_val -> Prop)
+  (P_exp_val : exp_val -> Prop).
+
+Hypothesis
+  (H_EV_Bits : forall (bv5:string), forall (annot5:unit), P_exp_val (EV_Bits bv5 annot5))
+  (H_EV_Bool : forall (bool5:bool), forall (annot5:unit), P_exp_val (EV_Bool bool5 annot5))
+  (H_EV_Enum : forall (enum5:enum), forall (annot5:unit), P_exp_val (EV_Enum enum5 annot5))
+  (H_EV_Unop : forall (unop5:unop), forall (exp_val5:exp_val), P_exp_val exp_val5 -> forall (annot5:unit), P_exp_val (EV_Unop unop5 exp_val5 annot5))
+  (H_EV_Binop : forall (binop5:binop), forall (exp_val1:exp_val), P_exp_val exp_val1 -> forall (exp_val2:exp_val), P_exp_val exp_val2 -> forall (annot5:unit), P_exp_val (EV_Binop binop5 exp_val1 exp_val2 annot5))
+  (H_EV_Manyop : forall (exp_val_list:list exp_val), P_list_exp_val exp_val_list -> forall (manyop5:manyop), forall (annot5:unit), P_exp_val (EV_Manyop manyop5 exp_val_list annot5))
+  (H_EV_Ite : forall (exp_val1:exp_val), P_exp_val exp_val1 -> forall (exp_val2:exp_val), P_exp_val exp_val2 -> forall (exp_val3:exp_val), P_exp_val exp_val3 -> forall (annot5:unit), P_exp_val (EV_Ite exp_val1 exp_val2 exp_val3 annot5))
+  (H_list_exp_val_nil : P_list_exp_val nil)
+  (H_list_exp_val_cons : forall (exp_val0:exp_val), P_exp_val exp_val0 -> forall (exp_val_l:list exp_val), P_list_exp_val exp_val_l -> P_list_exp_val (cons exp_val0 exp_val_l)).
+
+Fixpoint exp_val_ott_ind (n:exp_val) : P_exp_val n :=
+  match n as x return P_exp_val x with
+  | (EV_Bits bv5 annot5) => H_EV_Bits bv5 annot5
+  | (EV_Bool bool5 annot5) => H_EV_Bool bool5 annot5
+  | (EV_Enum enum5 annot5) => H_EV_Enum enum5 annot5
+  | (EV_Unop unop5 exp_val5 annot5) => H_EV_Unop unop5 exp_val5 (exp_val_ott_ind exp_val5) annot5
+  | (EV_Binop binop5 exp_val1 exp_val2 annot5) => H_EV_Binop binop5 exp_val1 (exp_val_ott_ind exp_val1) exp_val2 (exp_val_ott_ind exp_val2) annot5
+  | (EV_Manyop manyop5 exp_val_list annot5) => H_EV_Manyop exp_val_list (((fix exp_val_list_ott_ind (exp_val_l:list exp_val) : P_list_exp_val exp_val_l := match exp_val_l as x return P_list_exp_val x with nil => H_list_exp_val_nil | cons exp_val1 xl => H_list_exp_val_cons exp_val1(exp_val_ott_ind exp_val1)xl (exp_val_list_ott_ind xl) end)) exp_val_list) manyop5 annot5
+  | (EV_Ite exp_val1 exp_val2 exp_val3 annot5) => H_EV_Ite exp_val1 (exp_val_ott_ind exp_val1) exp_val2 (exp_val_ott_ind exp_val2) exp_val3 (exp_val_ott_ind exp_val3) annot5
+end.
+
+End exp_val_rect.
 
 
 (**********************************)
@@ -322,10 +373,43 @@ Record sequential_state := {
 
 
 Fixpoint valu_eqb (v1 v2 : valu) : bool :=
-    match v1, v2 with
-    | Val_Bool b1, Val_Bool b2 => Bool.eqb b1 b2
-    | _, _ => false (* TODO: other cases *)
-    end.
+  match v1, v2 with
+  | Val_Bool b1, Val_Bool b2 => Bool.eqb b1 b2
+  | _, _ => false (* TODO: other cases *)
+  end.
+
+Definition write_byte (addr : valu) (value : valu) (s : sequential_state)
+: sequential_state :=
+  {| seqst_reg_map := s.(seqst_reg_map);
+     seqst_mem_map := fun y => if valu_eqb addr y then Some value else s.(seqst_mem_map) y |}.
+
+(* It's not clear to me exactly how this should work *)
+Axiom split : valu -> valu * valu.
+
+(*
+Definition write_bytes
+  (addr : valu)
+  (sz : Z)
+  (value : valu)
+  (s : sequential_state)
+  : sequential_state.
+Proof.
+  Local Close Scope Z.
+  refine ((z_ind (fun x => valu -> sequential_state) _ _ sz) value).
+  + intros v'.
+    exact s.
+  + intros x H ind v'.
+    assert (v'' : mword (8 + 8*x)).
+    - refine (cast_T v' _).
+      apply eq_sym.
+      apply pluseight.
+    - pose (v''':=mword_split v'').
+      destruct v''' as [a b].
+      pose (s' := ind b).
+      pose (addr' := addr_offset addr (sz-x)).
+      exact (write_byte addr a s').
+Defined.
+*)
 
 Inductive sequential_state_step : sequential_state -> proper_label -> sequential_state -> Prop :=
 | seqststep_read_reg seqst r v :
